examples/hanoi/hanoi_dom.pddl
@@ -1,0 +1,21 @@
+(define (domain hanoi)
+(:requirements :adl :types)
+(:predicates (clear ?x)
+             (on ?x ?y)
+             (smaller ?x ?y))
+
+(:functions
+    (under ?x) - object
+)
+
+(:action move
+:parameters (?disc ?from ?to)
+:precondition (and (smaller ?to ?disc) 
+                   (on ?disc ?from) 
+                   (clear ?disc) 
+                   (clear ?to))
+:effect  (and (clear ?from) 
+              (on ?disc ?to) 
+              (not (on ?disc ?from))  
+              (not (clear ?to)))
+ )) 
